kk

examples/n_german/n_mutualEx_base.thy
@@ -5,72 +5,689 @@
 
 (*header{*The n_mutualEx Protocol Case Study*} *)
 
-theory n_mutualEx_base imports paraTheoryCmpzb
+theory n_mutualEx_base
+  imports paraTheoryCmpzb
 begin
 
-section{*Main definitions*}
+section \<open>Main definitions\<close>
 
-subsection{* Definitions of Constants*}
-definition I::"scalrValueType" where [simp]: "I\<equiv> enum ''control'' ''I''"
-definition T::"scalrValueType" where [simp]: "T\<equiv> enum ''control'' ''T''"
-definition C::"scalrValueType" where [simp]: "C\<equiv> enum ''control'' ''C''"
-definition E::"scalrValueType" where [simp]: "E\<equiv> enum ''control'' ''E''"
-definition true::"scalrValueType" where [simp]: "true\<equiv> boolV True"
-definition false::"scalrValueType" where [simp]: "false\<equiv> boolV False"
+subsection \<open>Definitions of Constants\<close>
+
+text \<open>Represents four states: idle, try, critical, exit\<close>
+definition I :: scalrValueType where [simp]: "I \<equiv> enum ''control'' ''I''"
+definition T :: scalrValueType where [simp]: "T \<equiv> enum ''control'' ''T''"
+definition C :: scalrValueType where [simp]: "C \<equiv> enum ''control'' ''C''"
+definition E :: scalrValueType where [simp]: "E \<equiv> enum ''control'' ''E''"
+
+definition true :: scalrValueType where [simp]: "true \<equiv> boolV True"
+definition false :: scalrValueType where [simp]: "false \<equiv> boolV False"
+
+axiomatization  where axiomOnf2 [simp,intro]:
+   "s  (Para ( ''n'') i) = I \<or> s  (Para ( ''n'') i) = T
+  \<or>s  (Para ( ''n'') i) = C \<or>s  (Para ( ''n'') i) = E"
+
+subsection \<open>Definitions of Parameterized Rules\<close>
+
+text \<open>If currently idle, can move to try
+  n[i] = I \<rightarrow> n[i] := T
+\<close>
+definition n_Try :: "nat \<Rightarrow> rule" where [simp]:
+  "n_Try i \<equiv>
+    let g = (eqn (IVar (Para ( ''n'') i)) (Const I)) in
+    let s = (parallelList [(assign ((Para ( ''n'') i), (Const T)))]) in
+      guard g s"
+
+text \<open>Enter critical region
+  n[i] = T \<and> x = True \<rightarrow> n[i] := C; x := False
+\<close>
+definition n_Crit :: "nat \<Rightarrow> rule" where [simp]:
+  "n_Crit i \<equiv>
+    let g = (andForm (eqn (IVar (Para ( ''n'') i)) (Const T)) (eqn (IVar (Ident ''x'')) (Const true))) in
+    let s = (parallelList [(assign ((Para ( ''n'') i), (Const C))), (assign ((Ident ''x''), (Const false)))]) in
+      guard g s"
+
+text \<open>Exit critical region
+  n[i] = C \<rightarrow> n[i] := E
+\<close>
+definition n_Exit::"nat \<Rightarrow> rule" where [simp]:
+  "n_Exit i \<equiv>
+    let g = (eqn (IVar (Para ( ''n'') i)) (Const C)) in
+    let s = (parallelList [(assign ((Para ( ''n'') i), (Const E)))]) in
+      guard g s"
+
+text \<open>Move to idle
+  n[i] = E \<rightarrow> n[i] := I; x := True
+\<close>
+definition n_Idle :: "nat \<Rightarrow> rule" where [simp]:
+  "n_Idle i \<equiv>
+    let g = (eqn (IVar (Para ( ''n'') i)) (Const E)) in
+    let s = (parallelList [(assign ((Para ( ''n'') i), (Const I))), (assign ((Ident ''x''), (Const true)))]) in
+      guard g s"
 
 
+subsection \<open>The set of all actual rules w.r.t. a protocol instance with size $N$\<close>
 
-subsection{*  Definitions of Parameterized Rules *}
+definition rules :: "nat \<Rightarrow> rule set" where [simp]:
+  "rules N \<equiv> {r.
+    (\<exists>i. i \<le> N \<and> r = n_Try i) \<or>
+    (\<exists>i. i \<le> N \<and> r = n_Crit i) \<or>
+    (\<exists>i. i \<le> N \<and> r = n_Exit i) \<or>
+    (\<exists>i. i \<le> N \<and> r = n_Idle i) 
+   }"
+
+lemma rulesIsSym:
+  shows "symProtRules N (rules N)"
+proof (simp only: symProtRules_def, (rule allI)+, rule impI)
+  fix p r
+  assume a1: "p permutes {x.   x \<le> N} \<and> r \<in> rules N"
+  show "applySym2Rule p r \<in> rules N"
+  proof -
+    have b1:
+     "(\<exists>i. i \<le> N \<and> r = n_Try i) \<or>
+      (\<exists>i. i \<le> N \<and> r = n_Crit i) \<or>
+      (\<exists>i. i \<le> N \<and> r = n_Exit i) \<or>
+      (\<exists>i. i \<le> N \<and> r = n_Idle i) "
+      using local.a1 by auto
+    moreover
+    {assume b1:"\<exists> i. i\<le>N\<and>r=n_Try  i"
+      from b1 obtain i where b1:"i\<le>N\<and>r=n_Try  i"
+        by blast
+      from a1 have b2:"p i \<le> N"
+        by (metis (mono_tags, lifting) b1 mem_Collect_eq permutes_def permutes_in_image)
+      from b1 have b3:"applySym2Rule p r= n_Try  ( p i)" 
+        by auto
+      have "applySym2Rule p r \<in> rules N "
+        by (simp add: b2 b3)
+    }
+    moreover
+    {assume b1:"\<exists> i. i\<le>N\<and>r=n_Crit  i"
+      from b1 obtain i where b1:"i\<le>N\<and>r=n_Crit  i"
+        by blast
+      from a1 have b2:"p i \<le> N"
+        by (metis (mono_tags, lifting) b1 mem_Collect_eq permutes_def permutes_in_image)
+      from b1 have b3:"applySym2Rule p r= n_Crit  ( p i)" 
+        by auto
+      have "applySym2Rule p r \<in> rules N "
+        by (simp add: b2 b3)
+    }
+    moreover
+    {assume b1:"\<exists> i. i\<le>N\<and>r=n_Idle  i"
+      from b1 obtain i where b1:"i\<le>N\<and>r=n_Idle  i"
+        by blast
+      from a1 have b2:"p i \<le> N"
+        by (metis (mono_tags, lifting) b1 mem_Collect_eq permutes_def permutes_in_image)
+      from b1 have b3:"applySym2Rule p r= n_Idle  ( p i)" 
+        by auto
+      have "applySym2Rule p r \<in> rules N "
+        by (simp add: b2 b3)
+    }
+    moreover
+    {assume b1:"\<exists> i. i\<le>N\<and>r=n_Exit  i"
+      from b1 obtain i where b1:"i\<le>N\<and>r=n_Exit  i"
+        by blast
+      from a1 have b2:"p i \<le> N"
+        by (metis (mono_tags, lifting) b1 mem_Collect_eq permutes_def permutes_in_image)
+      from b1 have b3:"applySym2Rule p r= n_Exit  ( p i)" 
+        by auto
+      have "applySym2Rule p r \<in> rules N "
+        by (simp add: b2 b3)
+    }
+    ultimately show "applySym2Rule p r \<in> rules N"
+      by blast
+  qed
+qed
+
+(*definition rules'::"nat \<Rightarrow> rule set" where [simp]:
+"rules' N \<equiv> {r.
+(\<exists> p. p permutes {x. 1 \<le> x \<and> x \<le> N} \<and>r=n_Try  (p 1)) \<or>
+(\<exists> p. p permutes {x. 1 \<le> x \<and> x \<le> N} \<and>r=n_Crit  (p 1)) \<or>
+(\<exists> p. p permutes {x. 1 \<le> x \<and> x \<le> N} \<and>r=n_Exit  (p 1)) \<or>
+(\<exists> p. p permutes {x. 1 \<le> x \<and> x \<le> N} \<and>r=n_Idle  (p 1)) 
+}"
+
+lemma rules'IsSym:
+  shows "symProtRules N (rules' N)"
+
+proof(simp only:symProtRules_def,(rule allI)+,rule impI)  *)
+
+subsection \<open>Definitions of a formally parameterized invariant formulas\<close>
+
+text \<open>If any process is in exit state, x must be False.
+  n[i] = E \<longrightarrow> x = False
+\<close>
+definition inv_27 :: "nat \<Rightarrow> formula" where [simp]:
+  "inv_27 i \<equiv>
+    (implyForm (eqn (IVar (Para ''n'' i)) (Const E)) (eqn (IVar (Ident ''x'')) (Const false)))"
+
+text \<open>No two processes can be in the exit state in the same time.
+  i \<noteq> j \<longrightarrow> n[i] = E \<longrightarrow> n[j] \<noteq> E
+\<close>
+definition inv_7 :: "nat \<Rightarrow> nat \<Rightarrow> formula" where [simp]:
+  "inv_7 i j \<equiv>
+    implyForm (andForm (neg (eqn (Const (index i)) (Const (index j)))) (eqn (IVar (Para ''n'' i)) (Const E))) 
+      (neg (eqn (IVar (Para ''n'' j)) (Const E)))"
+
+text \<open>There cannot be one state in exit and another in critical.
+  i \<noteq> j \<longrightarrow> n[i] = E \<longrightarrow> n[j] \<noteq> C
+\<close>
+definition inv_5 :: "nat \<Rightarrow> nat \<Rightarrow> formula" where [simp]:
+  "inv_5 i j \<equiv>
+    implyForm (andForm (neg (eqn (Const (index i)) (Const (index j))))  
+      (eqn (IVar (Para ''n'' i)) (Const E))) (neg (eqn (IVar (Para ''n'' j)) (Const C)))"
+
+
+subsection \<open>Definitions of the set of invariant formula instances in a $N$-protocol instance\<close>
+
+definition invariants :: "nat \<Rightarrow> formula set" where [simp]:
+  "invariants N \<equiv> {f.
+    (\<exists>i.   i \<le> N \<and> f = inv_27 i) \<or>
+    (\<exists>i j. i \<le> N \<and> j \<le> N \<and> i \<noteq> j \<and> f = inv_7 i j) \<or>
+    (\<exists>i j. i \<le> N \<and> j \<le> N \<and> i \<noteq> j \<and> f = inv_5 i j)
+   }" 
+
+text \<open>Initial condition: all processes in idle.
+  \<forall>i. n[i] = I
+\<close>
+definition initSpec0 :: "nat \<Rightarrow> formula" where [simp]:
+  "initSpec0 N \<equiv> forallForm (down N) (\<lambda>i. eqn (IVar (Para ''n'' i)) (Const I))"
+
+text \<open>Initial condition: x is True\<close>
+definition initSpec1 :: formula where [simp]:
+  "initSpec1 \<equiv> eqn (IVar (Ident ''x'')) (Const true)"
+
+definition allInitSpecs::"nat \<Rightarrow> formula list" where [simp]:
+  "allInitSpecs N \<equiv> [initSpec0 N, initSpec1]"
+
+subsection \<open>Definitions of the set of invariant formula used in each rule
+and each rule in middle protocol protPP\<close>
+
+definition n_Idle_Ls :: "nat \<Rightarrow> nat\<Rightarrow> formula list" where [simp]:
+  "n_Idle_Ls N i\<equiv> 
+  (map (\<lambda>j. if (i=j) then chaos else inv_7 i j) (down N)) @
+  (map (\<lambda>j. if (i=j) then chaos else inv_5 i j) (down N))"
+(*{f.
+    (\<exists> j.   j \<le> N \<and> i \<noteq> j \<and> f = inv_7 i j) \<or>
+    (\<exists> j.   j \<le> N \<and> i \<noteq> j \<and> f = inv_5 i j)}"*)
+
+definition n_Idle_PP :: "nat \<Rightarrow> nat\<Rightarrow>rule" where [simp]:
+  "n_Idle_PP N i\<equiv> strengthenR (n_Idle_Ls N i) (n_Idle i)"
+
+definition rulesOfPP :: "nat \<Rightarrow> rule set" where [simp]:
+  "rulesOfPP N \<equiv> {r.
+    (\<exists>i. i \<le> N \<and> r = n_Try i) \<or>
+    (\<exists>i. i \<le> N \<and> r = n_Crit i) \<or>
+    (\<exists>i. i \<le> N \<and> r = n_Exit i) \<or>
+    (\<exists>i. i \<le> N \<and> r = n_Idle_PP N i) 
+   }"
+lemma onMapSetDown:
+  "set (map f (down N)) ={g. \<exists>j.  j\<le>N \<and> g= f j}"
+(*proof(induct_tac N,simp,auto) *)
+  sorry 
+lemma onMapStrenghthEnCat:
+  "and2ListF (strengthen (x#xs) g) = and2ListF (strengthenForm x g) \<union> (and2ListF (strengthen xs g))"
+  by (simp add: sup_left_commute)
+    
+lemma onMapStrenghthEnUn:
+  "and2ListF (strengthen (xs@ys) g) =
+  (and2ListF (strengthen (xs) g)) \<union> (and2ListF (strengthen ys g))"  (is "?P xs ys")
+proof(induct_tac xs)
+  show "?P [] ys"
+  proof(simp)qed
+next
+  fix x xs
+
+  assume a1:"?P xs ys"
+  show "?P (x#xs) ys"
+    using a1 by auto
+qed
+
+lemma onMapStrenghthEn:
+  "  and2ListF ( strengthen (map f (down N)) g) =
+  (and2ListF g) Un {g'. \<exists>j. j\<le>N   \<and> g' \<in> (and2ListF (strengthenForm (f j) g))  }" (is "?P N")
+proof(induct_tac N)
+  show "?P 0" 
+    by simp
+next
+  fix N
+  assume a1:"?P N"
+  show "?P (Suc N)"
+  proof -
+    have b1:"(map f (down (Suc N))) =map f ([Suc N]@(down N))"
+      by simp 
+    from b1  show  "?P (Suc N)"
+    proof( simp add:onMapStrenghthEnUn)  
+      show "and2ListF g \<union> (and2ListF (strengthenForm (f (Suc N)) g) \<union> and2ListF (strengthenFormByForms (map f (down N)) g)) = and2ListF g \<union> {g'. \<exists>j\<le>Suc N. g' \<in> and2ListF (strengthenForm (f j) g)}"
+        (is "?LHS = ?RHS")
+      proof
+        show "?LHS \<subseteq> ?RHS"
+        proof
+          fix x
+          assume c1:"x \<in> ?LHS "
+          show "x \<in> ?RHS"
+          proof -
+            have c2:"x \<in> and2ListF g | x \<in>(and2ListF (strengthenForm (f (Suc N)) g)) | x \<in>and2ListF (strengthenFormByForms (map f (down N)) g)  "
+              using c1 by blast
+            moreover
+            {assume d1:"x \<in> and2ListF g"
+              have "x \<in> ?RHS"
+                using d1  by blast
+            }
+            moreover
+            {assume d1:"x \<in>(and2ListF (strengthenForm (f (Suc N)) g))"
+              have "x \<in> ?RHS"
+                using d1  by blast
+            }
+            moreover
+            {assume d1:"x \<in>and2ListF (strengthenFormByForms (map f (down N)) g)"
+              have "x \<in> (and2ListF g) Un {g'. \<exists>j. j\<le>N   \<and> g' \<in> (and2ListF (strengthenForm (f j) g))  }"
+                apply(cut_tac a1,simp)
+                using a1 d1  by blast
+              then    have "x \<in> ?RHS"
+                by auto 
+            }
+            ultimately show "x \<in> ?RHS"
+              by blast
+          qed
+        qed
+      next
+        show "?RHS \<subseteq> ?LHS"
+        proof
+          fix x
+          assume c1:"x \<in> ?RHS "
+          show "x \<in> ?LHS"
+          proof -
+            have d1:" x \<in> and2ListF g | x \<in> {g'. \<exists>j\<le>Suc N. g' \<in> and2ListF (strengthenForm (f j) g)}"
+              using c1 by auto
+            moreover
+            {assume d1:"x \<in> and2ListF g "
+              have  "x \<in> ?LHS"
+                using d1 by blast
+            }
+            moreover
+            {assume d1:"x \<in> {g'. \<exists>j\<le>Suc N. g' \<in> and2ListF (strengthenForm (f j) g)} "
+              have  "x \<in> {g'.  g' \<in> and2ListF (strengthenForm (f (Suc N)) g)} | x \<in> {g'. \<exists>j\<le> N. g' \<in> and2ListF (strengthenForm (f j) g)}"
+                using d1 le_Suc_eq by force 
+              moreover
+              {assume d1:"x \<in> {g'.  g' \<in> and2ListF (strengthenForm (f (Suc N)) g)} "
+                have "x \<in> ?LHS"
+                  using d1 by auto
+              }
+              moreover
+              {assume d1:"  x \<in> {g'. \<exists>j\<le> N. g' \<in> and2ListF (strengthenForm (f j) g)} "
+                have "x \<in> ?LHS"
+                  using a1 calculation(1) by auto 
+              }
+            ultimately have "x \<in> ?LHS"
+              by blast
+          }
+          ultimately show "x \<in> ?LHS"
+              by blast
+          qed
+        qed
+      qed
+    qed
+  qed
+qed
+
+lemma tautSYm: assumes a1:"p permutes {i.  i \<le> N}"
+  shows "taut f= taut (applySym2Form p f)"
+proof
+  assume b1:"taut f"
+  show "taut (applySym2Form p (f))"
+  proof(unfold taut_def,rule allI)
+    fix s
+    have b2:"formEval f ( (applySym2State (inv p) s))"
+      by(cut_tac b1,auto) 
+    have b3:"formEval (applySym2Form  p f) (applySym2State p (applySym2State (inv p) s)) = formEval f ( (applySym2State (inv p) s))"
+      using stFormSymCorrespondence a1 by auto
+    have b4:"bij p"
+      using a1 permutes_bij by blast
+      
+    have b5:"applySym2State p (applySym2State (inv p) s) =s "
+    proof
+      fix x
+      show "applySym2State p (applySym2State (inv p) s) x  =s x"
+        using b4  applySym2StateInv by blast 
+    qed
+    with b2 b5 b3 show "formEval (applySym2Form  p f) s"
+      by auto
+  qed
+next
+  assume b1:"taut (applySym2Form p (f)) "
+  show "taut f"
+  proof(unfold taut_def,rule allI)
+    fix s
+    have b2:"formEval (applySym2Form p (f)) ( (applySym2State p s))"
+      by(cut_tac b1,auto) 
+    have b4:"bij p"
+      using a1 permutes_bij by blast
+    then show "formEval f s"
+      using assms b2 stFormSymCorrespondence by auto
+  qed
+qed
+
+lemma onStrengthenFormSymApp:
+  assumes a1:"p permutes {i. i \<le> N}"
+  shows "applySym2Form p (strengthenForm x g) = strengthenForm (applySym2Form p x) (applySym2Form p g)"
+  (is "?LHS=?RHS")
+proof(case_tac x)
+  fix ant0 cons0
+  assume b1:"x=implyForm ant0 cons0"  
+  have "taut (implyForm g ant0) | \<not> taut (implyForm g ant0)" 
+    by blast
+  moreover
+  {assume b2:"taut (implyForm g ant0)"
+    have b3:"applySym2Form p (strengthenForm x g) =applySym2Form p (cons0)"  
+       by(cut_tac b1 b2, simp)
+     from b2 have b4:"taut (applySym2Form p (implyForm g ant0))"
+       using a1 tautSYm by blast
+     then have b5:"taut (implyForm (applySym2Form p g) (applySym2Form p ant0))"
+       by simp
+     with b1  have "strengthenForm (applySym2Form p x) (applySym2Form p g) =
+          applySym2Form p (cons0)"
+       by simp
+     with b3 have "?LHS=?RHS"
+       by simp
+   }
+  moreover
+  {assume b2:"\<not>taut (implyForm g ant0)"
+    have b3:"applySym2Form p (strengthenForm x g) =chaos"
+      by(cut_tac b1 b2, auto)
+    from b2 have b4:"\<not>taut (applySym2Form p (implyForm g ant0))"
+       using a1 tautSYm by blast
+     then have b5:"~taut (implyForm (applySym2Form p g) (applySym2Form p ant0))"
+       by simp  
+    with b1  have "strengthenForm (applySym2Form p x) (applySym2Form p g) =
+          chaos"
+      by auto 
+     with b3 have "?LHS=?RHS"
+       by simp
+   }
+   ultimately show "?LHS=?RHS"
+     by blast
+ qed(auto)
+
+
+lemma  onMapStrenghthEnSymApp:
+  assumes a1:"p permutes {i. i \<le> N}"
+  shows
+  "and2ListF (applySym2Form p (strengthen Fs g) ) =
+  and2ListF (strengthen (map (applySym2Form p) Fs) (applySym2Form p g))" (is "?P Fs")
+proof(induct_tac Fs)
+  show "?P []"
+    by auto
+next
+  fix x xs
+  assume a1:"?P (xs)"
+  show "?P (x#xs)"  (is "?LHS = ?RHS")
+  proof-
+    have b1:"?LHS = and2ListF (applySym2Form p g) \<union> 
+    (and2ListF (applySym2Form p (strengthenForm x g)) \<union> 
+    and2ListF (applySym2Form p (strengthenFormByForms xs g))) "
+      by simp
+    have b2:"?RHS= and2ListF (applySym2Form p g) \<union> 
+    (and2ListF (strengthenForm (applySym2Form p x) (applySym2Form p g)) \<union> 
+    and2ListF (strengthenFormByForms (map (applySym2Form p) xs) (applySym2Form p g)))"
+      apply(simp add:onMapStrenghthEnUn onMapStrenghthEn)
+      done
+    have b3:"(applySym2Form p (strengthenForm x g)) =
+       (strengthenForm (applySym2Form p x) (applySym2Form p g)) "
+      using assms onStrengthenFormSymApp by auto
+      
+    show "?LHS =?RHS"
+      using b1 b2 b3 a1 onStrengthenFormSymApp by auto
+  qed
+qed
+
+lemma and2ListForall:
+  "(\<forall>f. f \<in>and2ListF g \<longrightarrow> formEval f s) = formEval g s"
+  
+lemma and2ListFCong:
+  shows a1:"and2ListF g1=and2ListF g2 \<longrightarrow> formEval  g1 s=formEval  g2 s"
+   
+  sorry
+
+
+lemma reachSymLemma':
+  assumes a1: "symPredList N fs"
+    and a2: "symProtRules' N rs" 
+      (*a3:"s \<in> reachableSetUpTo (andList fs) rs i " and*)
+    and a4: "p permutes {x.   x \<le> N}"
+  shows
+    "\<forall>s. s \<in> reachableSetUpTo (andList fs) rs i \<longrightarrow>
+         applySym2State p s \<in> reachableSetUpTo (andList fs) rs i" (is "?P i")
+proof (induct_tac i)
+  show "?P 0"
+  proof (rule allI,simp,rule impI,rule andListForm2,rule allI,rule impI)
+    fix s f
+    assume b1:"formEval (andList fs) s " and
+    b2:"f \<in> set fs"
+    have "(applySym2Form (inv p) f) \<in> set fs "
+      by (meson a1 a4 b2 permutes_inv symPredList_def)
+    then have b3:" formEval (applySym2Form (inv p) f) s"
+      using b1 by blast 
+    show "formEval f (applySym2State p s)"
+      by (metis (no_types, lifting) 
+          Collect_cong a4 applySym2ExpFormInv b3 bij_def permutes_inj 
+          permutes_inv_o(1) stFormSymCorrespondence surj_iff)
+  qed
+next
+  fix n
+  assume b1:"?P n"
+  show "?P (Suc n)"
+  proof
+    fix s
+    show "s \<in> reachableSetUpTo (andList fs) rs (Suc n) \<longrightarrow> applySym2State p s \<in> reachableSetUpTo (andList fs) rs (Suc n)"
+    proof
+    assume c1:"s \<in> reachableSetUpTo (andList fs) rs (Suc n)"
+    from c1 have c2:"s \<in> reachableSetUpTo (andList fs) rs ( n) \<or>
+      (\<exists> s0 r. s0 \<in> reachableSetUpTo (andList fs)  rs n \<and> r \<in> rs \<and> 
+        formEval (pre r) s0 \<and>s = trans1 (act r) s0)"
+      by auto
+    moreover
+    {assume c2:"s \<in> reachableSetUpTo (andList fs) rs ( n)"
+      have c3:"applySym2State p s \<in> reachableSetUpTo (andList fs) rs ( n)"
+        using b1 c2 by blast
+      have "
+    applySym2State p s \<in> reachableSetUpTo (andList fs) rs (Suc n)"
+        by (simp add: c3)
+    }
+    moreover
+    {assume c2:" (\<exists> s0 r. s0 \<in> reachableSetUpTo (andList fs)  rs n \<and> r \<in> rs \<and> 
+        formEval (pre r) s0 \<and>s = trans1 (act r) s0)"
+      then obtain s0 r where c2:"s0 \<in> reachableSetUpTo (andList fs)  rs n \<and> r \<in> rs \<and> 
+        formEval (pre r) s0 \<and>s = trans1 (act r) s0"
+        by blast
+
+      from b1 c1 have c3:"applySym2State p s0 \<in> reachableSetUpTo (andList fs) rs ( n)"
+        using b1 c2 by blast
+      have c4:"formEval (applySym2Form p (pre  r)) (applySym2State p s0)"
+        using a4 c2 stFormSymCorrespondence by auto
+       
+      have c5:" applySym2Form p (pre  r) = pre (applySym2Rule p r)"
+        apply(case_tac "r",auto) done
+      with c4 have c6:"formEval ( pre (applySym2Rule p r)) (applySym2State p s0)"
+        by simp
+      
+      have c7:"\<exists>r'. alphaEqRule r'( applySym2Rule p r) \<and>r' \<in> rs"
+        using a2 a4 c2 symProtRules'_def by blast
+      then obtain r' where c7:" alphaEqRule r'( applySym2Rule p r) \<and>r' \<in> rs"
+        by blast
+
+      from c6 c7 have c7a:"formEval ( pre r') (applySym2State p s0)"
+        by (simp add: c6 and2ListFCong)
+        
+      have c8:"applySym2State p (trans1 (act r) s0) =
+          trans1 (act (applySym2Rule p r)) (applySym2State p s0)"
+        by (metis a4 act.simps applySym2Rule.simps rule.exhaust transSym)
+
+      have c9:"trans1 (act r' ) (applySym2State p s0) \<in>  reachableSetUpTo (andList fs) rs (Suc n)"
+        using c3 c7 c7a  by fastforce 
+
+       have c9a:"trans1 (act r' ) (applySym2State p s0) = trans1 (act (applySym2Rule p r)) (applySym2State p s0)"
+        using c3 c7 c7a  by fastforce 
+
+      have "applySym2State p s \<in> reachableSetUpTo (andList fs) rs (Suc n)"
+        using c2 c8 c9 c9a by auto 
+    } 
+    ultimately show "applySym2State p s \<in> reachableSetUpTo (andList fs) rs (Suc n)"
+      by blast
+  qed
+qed
+qed
+
+
+lemma SymLemma':
+  assumes a1: "symPredList N fs"
+    and a2: "symProtRules' N rs"
+    and a3: "\<forall>s i. s \<in> reachableSetUpTo (andList fs) rs i \<longrightarrow> formEval f s"
+    and a4: "p permutes {x.   x \<le> N}"
+  shows
+    "\<forall>s i. s \<in> reachableSetUpTo (andList fs) rs i \<longrightarrow> formEval (applySym2Form p f) s" (is "?P i")
+
+lemma rulesOfPPIsSym:
+  shows "symProtRules N (rulesOfPP N)"
+proof (simp only: symProtRules_def, (rule allI)+, rule impI)
+  fix p r
+  assume a1:"p permutes {x.   x \<le> N} \<and> r \<in> rulesOfPP N "
+  show "applySym2Rule p r \<in> rulesOfPP N"
+  proof -
+    have b1: 
+     "(\<exists>i. i \<le> N \<and> r = n_Try i) \<or>
+      (\<exists>i. i \<le> N \<and> r = n_Crit i) \<or>
+      (\<exists>i. i \<le> N \<and> r = n_Exit i) \<or>
+      (\<exists>i. i \<le> N \<and> r = n_Idle_PP N i)"
+      using local.a1 by auto
+    moreover
+    {assume b1:"\<exists> i. i\<le>N\<and>r=n_Try  i"
+      from b1 obtain i where b1:"i\<le>N\<and>r=n_Try  i"
+        by blast
+      from a1 have b2:"p i \<le> N"
+        by (metis (mono_tags, lifting) b1 mem_Collect_eq permutes_def permutes_in_image)
+      from b1 have b3:"applySym2Rule p r= n_Try  ( p i)" 
+        by auto
+      have "applySym2Rule p r \<in> rules N "
+        by (simp add: b2 b3)
+    }   
+    moreover
+    {assume b1:"\<exists> i. i\<le>N\<and>r=n_Crit  i"
+      from b1 obtain i where b1:"i\<le>N\<and>r=n_Crit  i"
+        by blast
+      from a1 have b2:"p i \<le> N"
+        by (metis (mono_tags, lifting) b1 mem_Collect_eq permutes_def permutes_in_image)
+      from b1 have b3:"applySym2Rule p r= n_Crit  ( p i)" 
+        by auto
+      have "applySym2Rule p r \<in> rules N "
+        by (simp add: b2 b3)
+    }
+    moreover
+    {assume b1:"\<exists> i. i\<le>N\<and>r=n_Idle_PP N  i"
+      from b1 obtain i where b1:"i\<le>N\<and>r=n_Idle_PP N i"
+        by blast
+      from a1 have b2:"p i \<le> N"
+        by (metis (mono_tags, lifting) b1 mem_Collect_eq permutes_def permutes_in_image)
+      have b3:"p permutes {x.   x \<le> N}" sorry
+      have b4:"and2ListF (pre ( n_Idle_PP N (p i))) =
+               and2ListF ((strengthen (n_Idle_Ls N i)  (pre (n_Idle i))))" sorry
+      have b5:" and2ListF ((strengthen (n_Idle_Ls N (p i))  (pre (n_Idle (p i))))) =
+            { eqn (IVar (Para ''n'' (p i))) (Const (enum ''control'' ''E''))} \<union>
+               {f. \<exists>j. j\<le>N \<and> j\<noteq>p i \<and>f=conclude (inv_7 (p i) j)}\<union>
+               {f. \<exists>j. j\<le>N \<and> j\<noteq>p i \<and>f=conclude (inv_5 (p i) j)}"         
+        apply(   simp add:n_Idle_PP_def n_Idle_Ls_def n_Idle_def onMapStrenghthEn 
+                      onMapStrenghthEnUn del:strengthen_def,auto
+                      )
+        apply force
+        by (smt Collect_cong)
+
+(*
+{ eqn (IVar (Para ''n'' (p i))) (Const (enum ''control'' ''E''))} \<union>
+               {f. \<exists>j. j\<le>N \<and> j\<noteq>p i \<and>f=conclude (inv_7 (p i) j)}\<union>
+               {f. \<exists>j. j\<le>N \<and> j\<noteq>p i \<and>f=conclude (inv_5 (p i) j)}
+                
+              "*)
+      have b5:"and2ListF (pre (applySym2Rule p (n_Idle_PP N i))) =
+          { eqn (IVar (Para ''n'' (p i))) (Const (enum ''control'' ''E''))} \<union>
+               {f. \<exists>j. j\<le>N \<and> j\<noteq>p i \<and>f=conclude (inv_7 (p i) j)}\<union>
+               {f. \<exists>j. j\<le>N \<and> j\<noteq>p i \<and>f=conclude (inv_5 (p i) j)}
+                
+              "
+
+         apply(cut_tac b3,  simp add:n_Idle_PP_def n_Idle_Ls_def n_Idle_def onMapStrenghthEn 
+                      onMapStrenghthEnUn  onMapStrenghthEnSymApp
+                     del:strengthen_def,auto   )
+        apply (metis mem_Collect_eq permutes_def)
+        using permutes_in_image apply fastforce
+        apply auto[1]
+        apply (metis mem_Collect_eq permutes_def)
+        apply auto[1]
+        by (metis mem_Collect_eq permutes_def)
+         
+       
+      have b3:"alphaEqForm (pre (applySym2Rule p (n_Idle_PP N i)))(pre ( n_Idle_PP N (p i)))"
+        
+      have "applySym2Rule p r \<in> rules N"
+        sorry
+    }
+    moreover
+    {assume b1:"\<exists> i. i\<le>N\<and>r=n_Exit  i"
+      from b1 obtain i where b1:"i\<le>N\<and>r=n_Exit  i"
+        by blast
+      from a1 have b2:"p i \<le> N"
+        by (metis (mono_tags, lifting) b1 mem_Collect_eq permutes_def permutes_in_image)
+      from b1 have b3:"applySym2Rule p r= n_Exit  ( p i)" 
+        by auto
+      have "applySym2Rule p r \<in> rules N "
+        by (simp add: b2 b3)
+    }
+    ultimately show "applySym2Rule p r \<in> rulesOfPP N"
+      sorry
+  qed
+qed
+
+
+axiomatization  where axiomOnf2 [simp,intro]:
+   "s \<in> reachableSet (set (allInitSpecs N )) (rules N) \<Longrightarrow> 
+ 1 < N \<Longrightarrow> 1 < i \<Longrightarrow> j<2 \<Longrightarrow>  formEval (f 0 1) s \<Longrightarrow> formEval (f i j) s"
+
+
+subsection{*Definitions of  the Set of Abs Invariant Formula Instances *}
+definition invariantsAbs  ::"  nat \<Rightarrow> formula list" where [simp]:
+"invariantsAbs  i \<equiv> [
+inv_27 i ,
+inv_7 i 1 ,
+inv_7 i 0 ,
+inv_5 i 0 ,
+inv_5 i 1
+]"
+
+lemma mutualExPPSimmutualEx:
+  assumes a1:"\<forall>r. r \<in> rs \<longrightarrow>(\<exists> Ls . set Ls \<subseteq> set S \<and>  strengthenR Ls r \<in> rs')" and
+  a2:"\<forall>i s f. s \<in>reachableSetUpTo I rs' i \<longrightarrow> f \<in>set S \<longrightarrow>formEval f s" 
+shows "\<forall>s f. s \<in>reachableSetUpTo I rs i \<longrightarrow>
+   f \<in>set S \<longrightarrow>(s \<in>reachableSetUpTo I rs' i \<and>formEval f s)" (is "?P i")
+subsection{*Definitions of each abstracted rule*}
 
 definition  NC::"nat " where [simp]: "NC==1"
 
- definition VF::"varType set" where [simp]: 
-"VF \<equiv>{(Para ( ''n'') 0),(Para ( ''n'') 1),(Ident ''x'')}"
-definition n_Try::"nat \<Rightarrow> rule" where [simp]:
-"n_Try  i\<equiv>
-let g = (eqn (IVar (Para ( ''n'') i)) (Const I)) in
-let s = (parallelList [(assign ((Para ( ''n'') i), (Const T)))]) in
-guard g s"
-
-definition n_Crit::"nat \<Rightarrow> rule" where [simp]:
-"n_Crit  i\<equiv>
-let g = (andForm (eqn (IVar (Para ( ''n'') i)) (Const T)) (eqn (IVar (Ident ''x'')) (Const true))) in
-let s = (parallelList [(assign ((Para ( ''n'') i), (Const C))), (assign ((Ident ''x''), (Const false)))]) in
-guard g s"
-
-definition n_Exit::"nat \<Rightarrow> rule" where [simp]:
-"n_Exit  i\<equiv>
-let g = (eqn (IVar (Para ( ''n'') i)) (Const C)) in
-let s = (parallelList [(assign ((Para ( ''n'') i), (Const E)))]) in
-guard g s"
-
-definition n_Idle::"nat \<Rightarrow> rule" where [simp]:
-"n_Idle  i\<equiv>
-let g = (eqn (IVar (Para ( ''n'') i)) (Const E)) in
-let s = (parallelList [(assign ((Para ( ''n'') i), (Const I))), (assign ((Ident ''x''), (Const true)))]) in
-guard g s"
-
-definition n_Crit_i_3::"rule" where [simp]:
-"n_Crit_i_3  \<equiv>
-let g = (eqn (IVar (Ident ''x'')) (Const true)) in
-let s = (parallelList [(assign ((Ident ''x''), (Const false)))]) in
-guard g s"
-
-definition n_Idle_i_3::"rule" where [simp]:
-"n_Idle_i_3  \<equiv>
+definition n_Idle_abs::"rule" where [simp]:
+"n_Idle_abs  \<equiv>
 let g = (andForm (andForm (eqn (IVar (Ident ''x'')) (Const false)) 
 (forallForm (down NC) (\<lambda>j. (neg (eqn (IVar (Para ( ''n'') j)) (Const E))))))
  (forallForm (down NC) (\<lambda>j. (neg (eqn (IVar (Para ( ''n'') j)) (Const C)))))) in
 let s = (parallelList [(assign ((Ident ''x''), (Const true)))]) in
 guard g s"
 
-definition n_Idle_i_3PP::"nat \<Rightarrow> rule" where [simp]:
-"n_Idle_i_3PP i \<equiv>
-let g = andForm (eqn (IVar (Para ( ''n'') i)) (Const E)) (andForm (andForm (eqn (IVar (Ident ''x'')) (Const false)) 
-(forallForm (down NC) (\<lambda>j. (neg (eqn (IVar (Para ( ''n'') j)) (Const E))))))
- (forallForm (down NC) (\<lambda>j. (neg (eqn (IVar (Para ( ''n'') j)) (Const C)))))) in
-let s = (parallelList [(assign ((Ident ''x''), (Const true)))]) in
+
+
+ 
+
+definition n_Crit_abs::"rule" where [simp]:
+"n_Crit_abs  \<equiv>
+let g = (eqn (IVar (Ident ''x'')) (Const true)) in
+let s = (parallelList [(assign ((Ident ''x''), (Const false)))]) in
 guard g s"
+
+
 
 subsection{*The set of All actual Rules w.r.t. a Protocol Instance with Size $N$*}
 definition rules::"nat \<Rightarrow> rule set" where [simp]:
@@ -85,54 +702,15 @@ definition rules::"nat \<Rightarrow> rule set" where [simp]:
 
 
 
-subsection{*Definitions of a Formally Parameterized Invariant Formulas*}
 
-definition inv_27::"nat \<Rightarrow> formula" where [simp]:
-"inv_27 i \<equiv>
-(implyForm (eqn (IVar (Para ( ''n'') i)) (Const E)) (eqn (IVar (Ident ''x'')) (Const false)))"
 
-definition inv_7::"nat \<Rightarrow> nat \<Rightarrow> formula" where [simp]:
-"inv_7 i j \<equiv>
-(implyForm (neg (eqn (Const (index i)) (Const (index j)))) (implyForm (eqn (IVar (Para ( ''n'') i)) (Const E)) (neg (eqn (IVar (Para ( ''n'') j)) (Const E)))))"
 
-definition inv_5::"nat \<Rightarrow> nat \<Rightarrow> formula" where [simp]:
-"inv_5 i j \<equiv>
-(implyForm (neg (eqn (Const (index i)) (Const (index j)))) (implyForm (eqn (IVar (Para ( ''n'') i)) (Const E)) (neg (eqn (IVar (Para ( ''n'') j)) (Const C)))))"
 
-subsection{*Definitions of  the Set of Invariant Formula Instances in a $N$-protocol Instance*}
-definition invariants::"nat \<Rightarrow> formula set" where [simp]:
-"invariants N \<equiv> {f.
-(\<exists> i. i\<le>N\<and>f=inv_27  i) \<or>
-(\<exists> i j. i\<le>N\<and>j\<le>N\<and>i~=j\<and>f=inv_7  i j) \<or>
-(\<exists> i j. i\<le>N\<and>j\<le>N\<and>i~=j\<and>f=inv_5  i j)
-}" 
-
-subsection{*Definitions of  the Set of Abs Invariant Formula Instances *}
-definition invariantsAbs  ::"  formula list" where [simp]:
-"invariantsAbs   \<equiv> [
-inv_27 0 ,
-inv_7 0 1 ,
-inv_7 1 0 ,
-inv_5 0 1 ,
-inv_5 1 0
-]"
-
-definition initSpec0::"nat \<Rightarrow> formula" where [simp]:
-"initSpec0 N \<equiv> (forallForm (down N) (% i . (eqn (IVar (Para ( ''n'') i)) (Const I))))"
-
-definition initSpec1::"formula" where [simp]:
-"initSpec1  \<equiv> (eqn (IVar (Ident ''x'')) (Const true))"
-
-definition allInitSpecs::"nat \<Rightarrow> formula list" where [simp]:
-"allInitSpecs N \<equiv> [
-(initSpec0 N),
-(initSpec1 )
-]"
 axiomatization  where axiomOnf2 [simp,intro]:
-   "s ∈ reachableSet (set (allInitSpecs N )) (rules N) ⟹  1 < N ⟹ 1 < i ⟹ j<2 ⟹  formEval (f 0 1) s ⟹ formEval (f i j) s"
+   "s \<in> reachableSet (set (allInitSpecs N )) (rules N) \<Longrightarrow>  1 < N \<Longrightarrow> 1 < i \<Longrightarrow> j<2 \<Longrightarrow>  formEval (f 0 1) s \<Longrightarrow> formEval (f i j) s"
 
 axiomatization  where axiomOnf1 [simp,intro]:
-   "s ∈ reachableSet (set (allInitSpecs N )) (rules N) ⟹ 1 < N ⟹ 1 < i ⟹formEval (f 0 ) s ⟹ formEval (f i) s"
+   "s \<in> reachableSet (set (allInitSpecs N )) (rules N) \<Longrightarrow> 1 < N \<Longrightarrow> 1 < i \<Longrightarrow>formEval (f 0 ) s \<Longrightarrow> formEval (f i) s"
 
 
 
@@ -140,8 +718,8 @@ axiomatization  where axiomOnf1 [simp,intro]:
 subsection{*Definitions of initial states*}
 
 lemma lemmaOnn_TryGt_i:
-  assumes a1:"NC<i" and a2:"s ∈ reachableSet (set (allInitSpecs N)) (rules N)"  and  
-  a4:"∀f.  f ∈(set invariantsAbs) ⟶  formEval f s" 
+  assumes a1:"NC<i" and a2:"s \<in> reachableSet (set (allInitSpecs N)) (rules N)"  and  
+  a4:"\<forall>f.  f \<in>(set invariantsAbs) \<longrightarrow>  formEval f s" 
 shows "trans_sim_on2 (n_Try  i  ) skipRule VF (set invariantsAbs) s" (is "trans_sim_on2 ?r ?r' VF ?F s")
 proof(unfold trans_sim_on2_def,(rule allI)+,(rule impI)+,rule disjI2)
   fix s2 
@@ -150,7 +728,7 @@ proof(unfold trans_sim_on2_def,(rule allI)+,(rule impI)+,rule disjI2)
   proof(cut_tac a1,unfold state_sim_on2_def,
     (rule allI)+,(rule impI)+)
     fix f v
-    assume b1:" v ∈  VF"  
+    assume b1:" v \<in>  VF"  
     
     have b5:"trans (act (n_Try  i)) s v = s v" 
       by (cut_tac a1  b1,auto) 
@@ -165,25 +743,25 @@ lemma lemmaOnn_TryLeNc_:
   assumes a1:"i\<le>NC" 
   shows "trans_sim_on2 (n_Try  i) (n_Try  i) VF  (set invariantsAbs) s" (is "trans_sim_on2 ?r ?r VF ?F s")
 proof(rule ruleSimId2)
-  show  "∀v. v∈varOfForm (pre ?r) ⟶  v ∈ VF "
+  show  "\<forall>v. v\<in>varOfForm (pre ?r) \<longrightarrow>  v \<in> VF "
     by(cut_tac a1, auto) 
     
 next
-  show  b1: "∀v a. a ∈ set (statement2Assigns (act ?r)) ⟶ v∈varOfExp ( substExpByStatement (IVar (fst a))  (act ?r))⟶v ∈VF "
+  show  b1: "\<forall>v a. a \<in> set (statement2Assigns (act ?r)) \<longrightarrow> v\<in>varOfExp ( substExpByStatement (IVar (fst a))  (act ?r))\<longrightarrow>v \<in>VF "
    proof(cut_tac a1,(rule allI)+,(rule impI)+,auto) qed
     
  qed
 lemma lemmaOnn_Try: 
-  assumes   a2:"s ∈ reachableSet (set (allInitSpecs N)) (rules N)"  and  
-  a4:"∀f.  f ∈(set invariantsAbs) ⟶  formEval f s" and a5:"\<exists> i. i\<le>N\<and>r=n_Try  i"  and
+  assumes   a2:"s \<in> reachableSet (set (allInitSpecs N)) (rules N)"  and  
+  a4:"\<forall>f.  f \<in>(set invariantsAbs) \<longrightarrow>  formEval f s" and a5:"\<exists> i. i\<le>N\<and>r=n_Try  i"  and
   a6:"NC<N"
-  shows "∃ r'. r' ∈ rules NC∧ trans_sim_on2 r r' VF (set invariantsAbs) s" (is "∃r'.?P1 r' ∧ ?P2 r'")
+  shows "\<exists> r'. r' \<in> rules NC\<and> trans_sim_on2 r r' VF (set invariantsAbs) s" (is "\<exists>r'.?P1 r' \<and> ?P2 r'")
 proof -
   from a5 obtain i where d0:"i\<le>N\<and>r=n_Try  i"  by blast
   have "i>NC|i\<le> NC" by auto
   moreover{
        assume a1:"i>NC" 
-        have "∃r'. ?P1 r' ∧ ?P2 r'"
+        have "\<exists>r'. ?P1 r' \<and> ?P2 r'"
         proof(rule_tac x="(skipRule)" in exI,rule conjI)
           show  "?P1 (skipRule) " 
            by(cut_tac a1, auto) 
@@ -194,7 +772,7 @@ proof -
        }
 moreover{
        assume a1:"i\<le> NC" 
-        have "∃r'. ?P1 r' ∧ ?P2 r'"
+        have "\<exists>r'. ?P1 r' \<and> ?P2 r'"
         proof(rule_tac x="(n_Try  i)" in exI,rule conjI)
           show  "?P1 (n_Try  i) " 
            by(cut_tac a1, auto) 
@@ -203,17 +781,17 @@ moreover{
            using lemmaOnn_TryLeNc_ local.a1 a2 a4 a6 d0 by blast 
         qed
        }
-  ultimately show "∃r'.?P1 r' ∧ ?P2 r'" 
+  ultimately show "\<exists>r'.?P1 r' \<and> ?P2 r'" 
     by satx
 qed
 
 lemma lemmaOnn_CritGt_i:
   assumes a1:"i>NC" and 
-  a2:"s ∈ reachableSet (set (allInitSpecs N)) (rules N)"  and a3:"NC<N" and  
-  a4:"∀f.  f ∈(set invariantsAbs) ⟶  formEval f s" 
+  a2:"s \<in> reachableSet (set (allInitSpecs N)) (rules N)"  and a3:"NC<N" and  
+  a4:"\<forall>f.  f \<in>(set invariantsAbs) \<longrightarrow>  formEval f s" 
   shows "trans_sim_on2 (n_Crit  i)  (n_Crit_i_3 ) VF (set invariantsAbs) s" (is "trans_sim_on2 ?r ?r' VF (set ?F) s")
   proof(rule ruleSimCond2)
-    show " formEval (pre ?r) s ⟶formEval (pre ?r') s" (is "?A ⟶?B")
+    show " formEval (pre ?r) s \<longrightarrow>formEval (pre ?r') s" (is "?A \<longrightarrow>?B")
     proof(rule impI)+
       assume b0:"?A"
   
@@ -221,48 +799,48 @@ lemma lemmaOnn_CritGt_i:
        by auto
      qed
    next 
-	show "(∀  v. v ∈  varOfSent (act  ?r') ⟶  v ∈ VF ⟶ formEval (pre ?r) s ⟶ 
+	show "(\<forall>  v. v \<in>  varOfSent (act  ?r') \<longrightarrow>  v \<in> VF \<longrightarrow> formEval (pre ?r) s \<longrightarrow> 
     expEval (substExpByStatement (IVar v)  (act ?r')) s = expEval (substExpByStatement (IVar v)  (act ?r)) s)"
    proof(rule allI,(rule impI)+)
       fix  v
-     assume b1:"v∈ VF"  and b2:"formEval (pre ?r) s" and b3:"v ∈varOfSent (act ?r')"
+     assume b1:"v\<in> VF"  and b2:"formEval (pre ?r) s" and b3:"v \<in>varOfSent (act ?r')"
   
   show "expEval (substExpByStatement (IVar v)  (act ?r')) s = expEval (substExpByStatement (IVar v)  (act ?r)) s"  
        apply (cut_tac  a1 b1 b2 ,auto) done
    qed
  next
-   show "∀  v. v ∈  varOfSent (act ?r) ⟶  v ∈ VF ⟶ v ∈  varOfSent (act ?r')" by(cut_tac a1, auto)
+   show "\<forall>  v. v \<in>  varOfSent (act ?r) \<longrightarrow>  v \<in> VF \<longrightarrow> v \<in>  varOfSent (act ?r')" by(cut_tac a1, auto)
 
   
  next 
-   show "∀ v va. v ∈ varOfSent (act ?r') ⟶va∈varOfExp ( substExpByStatement (IVar v)  (act ?r'))⟶ va ∈ VF "
+   show "\<forall> v va. v \<in> varOfSent (act ?r') \<longrightarrow>va\<in>varOfExp ( substExpByStatement (IVar v)  (act ?r'))\<longrightarrow> va \<in> VF "
      by auto  
  next
-   show "∀v. v ∈ varOfForm (pre (?r')) ⟶ v ∈ VF" by auto
+   show "\<forall>v. v \<in> varOfForm (pre (?r')) \<longrightarrow> v \<in> VF" by auto
 qed
 lemma lemmaOnn_CritLeNc_:
   assumes a1:"i\<le>NC" 
   shows "trans_sim_on2 (n_Crit  i) (n_Crit  i) VF  (set invariantsAbs) s" (is "trans_sim_on2 ?r ?r VF ?F s")
 proof(rule ruleSimId2)
-  show  "∀v. v∈varOfForm (pre ?r) ⟶  v ∈ VF "
+  show  "\<forall>v. v\<in>varOfForm (pre ?r) \<longrightarrow>  v \<in> VF "
     by(cut_tac a1, auto) 
     
 next
-  show  b1: "∀v a. a ∈ set (statement2Assigns (act ?r)) ⟶ v∈varOfExp ( substExpByStatement (IVar (fst a))  (act ?r))⟶v ∈VF "
+  show  b1: "\<forall>v a. a \<in> set (statement2Assigns (act ?r)) \<longrightarrow> v\<in>varOfExp ( substExpByStatement (IVar (fst a))  (act ?r))\<longrightarrow>v \<in>VF "
    proof(cut_tac a1,(rule allI)+,(rule impI)+,auto) qed
     
  qed
 lemma lemmaOnn_Crit: 
-  assumes   a2:"s ∈ reachableSet (set (allInitSpecs N)) (rules N)"  and  
-  a4:"∀f.  f ∈(set invariantsAbs) ⟶  formEval f s" and a5:"\<exists> i. i\<le>N\<and>r=n_Crit  i"  and
+  assumes   a2:"s \<in> reachableSet (set (allInitSpecs N)) (rules N)"  and  
+  a4:"\<forall>f.  f \<in>(set invariantsAbs) \<longrightarrow>  formEval f s" and a5:"\<exists> i. i\<le>N\<and>r=n_Crit  i"  and
   a6:"NC<N"
-  shows "∃ r'. r' ∈ rules NC∧ trans_sim_on2 r r' VF (set invariantsAbs) s" (is "∃r'.?P1 r' ∧ ?P2 r'")
+  shows "\<exists> r'. r' \<in> rules NC\<and> trans_sim_on2 r r' VF (set invariantsAbs) s" (is "\<exists>r'.?P1 r' \<and> ?P2 r'")
 proof -
   from a5 obtain i where d0:"i\<le>N\<and>r=n_Crit  i"  by blast
   have "i>NC|i\<le> NC" by auto
   moreover{
        assume a1:"i>NC" 
-        have "∃r'. ?P1 r' ∧ ?P2 r'"
+        have "\<exists>r'. ?P1 r' \<and> ?P2 r'"
         proof(rule_tac x="(n_Crit_i_3 )" in exI,rule conjI)
           show  "?P1 (n_Crit_i_3 ) " 
            by(cut_tac a1, auto) 
@@ -273,7 +851,7 @@ proof -
        }
 moreover{
        assume a1:"i\<le> NC" 
-        have "∃r'. ?P1 r' ∧ ?P2 r'"
+        have "\<exists>r'. ?P1 r' \<and> ?P2 r'"
         proof(rule_tac x="(n_Crit  i)" in exI,rule conjI)
           show  "?P1 (n_Crit  i) " 
            by(cut_tac a1, auto) 
@@ -282,13 +860,13 @@ moreover{
            using lemmaOnn_CritLeNc_ local.a1 a2 a4 a6 d0 by blast 
         qed
        }
-  ultimately show "∃r'.?P1 r' ∧ ?P2 r'" 
+  ultimately show "\<exists>r'.?P1 r' \<and> ?P2 r'" 
     by satx
 qed
 
 lemma lemmaOnn_ExitGt_i:
-  assumes a1:"NC<i" and a2:"s ∈ reachableSet (set (allInitSpecs N)) (rules N)"  and  
-  a4:"∀f.  f ∈(set invariantsAbs) ⟶  formEval f s" 
+  assumes a1:"NC<i" and a2:"s \<in> reachableSet (set (allInitSpecs N)) (rules N)"  and  
+  a4:"\<forall>f.  f \<in>(set invariantsAbs) \<longrightarrow>  formEval f s" 
 shows "trans_sim_on2 (n_Exit  i  ) skipRule VF (set invariantsAbs) s" (is "trans_sim_on2 ?r ?r' VF ?F s")
 proof(unfold trans_sim_on2_def,(rule allI)+,(rule impI)+,rule disjI2)
   fix s2 
@@ -297,7 +875,7 @@ proof(unfold trans_sim_on2_def,(rule allI)+,(rule impI)+,rule disjI2)
   proof(cut_tac a1,unfold state_sim_on2_def,
     (rule allI)+,(rule impI)+)
     fix f v
-    assume b1:" v ∈  VF"  
+    assume b1:" v \<in>  VF"  
     
     have b5:"trans (act (n_Exit  i)) s v = s v" 
       by (cut_tac a1  b1,auto) 
@@ -312,25 +890,25 @@ lemma lemmaOnn_ExitLeNc_:
   assumes a1:"i\<le>NC" 
   shows "trans_sim_on2 (n_Exit  i) (n_Exit  i) VF  (set invariantsAbs) s" (is "trans_sim_on2 ?r ?r VF ?F s")
 proof(rule ruleSimId2)
-  show  "∀v. v∈varOfForm (pre ?r) ⟶  v ∈ VF "
+  show  "\<forall>v. v\<in>varOfForm (pre ?r) \<longrightarrow>  v \<in> VF "
     by(cut_tac a1, auto) 
     
 next
-  show  b1: "∀v a. a ∈ set (statement2Assigns (act ?r)) ⟶ v∈varOfExp ( substExpByStatement (IVar (fst a))  (act ?r))⟶v ∈VF "
+  show  b1: "\<forall>v a. a \<in> set (statement2Assigns (act ?r)) \<longrightarrow> v\<in>varOfExp ( substExpByStatement (IVar (fst a))  (act ?r))\<longrightarrow>v \<in>VF "
    proof(cut_tac a1,(rule allI)+,(rule impI)+,auto) qed
     
  qed
 lemma lemmaOnn_Exit: 
-  assumes   a2:"s ∈ reachableSet (set (allInitSpecs N)) (rules N)"  and  
-  a4:"∀f.  f ∈(set invariantsAbs) ⟶  formEval f s" and a5:"\<exists> i. i\<le>N\<and>r=n_Exit  i"  and
+  assumes   a2:"s \<in> reachableSet (set (allInitSpecs N)) (rules N)"  and  
+  a4:"\<forall>f.  f \<in>(set invariantsAbs) \<longrightarrow>  formEval f s" and a5:"\<exists> i. i\<le>N\<and>r=n_Exit  i"  and
   a6:"NC<N"
-  shows "∃ r'. r' ∈ rules NC∧ trans_sim_on2 r r' VF (set invariantsAbs) s" (is "∃r'.?P1 r' ∧ ?P2 r'")
+  shows "\<exists> r'. r' \<in> rules NC\<and> trans_sim_on2 r r' VF (set invariantsAbs) s" (is "\<exists>r'.?P1 r' \<and> ?P2 r'")
 proof -
   from a5 obtain i where d0:"i\<le>N\<and>r=n_Exit  i"  by blast
   have "i>NC|i\<le> NC" by auto
   moreover{
        assume a1:"i>NC" 
-        have "∃r'. ?P1 r' ∧ ?P2 r'"
+        have "\<exists>r'. ?P1 r' \<and> ?P2 r'"
         proof(rule_tac x="(skipRule)" in exI,rule conjI)
           show  "?P1 (skipRule) " 
            by(cut_tac a1, auto) 
@@ -341,7 +919,7 @@ proof -
        }
 moreover{
        assume a1:"i\<le> NC" 
-        have "∃r'. ?P1 r' ∧ ?P2 r'"
+        have "\<exists>r'. ?P1 r' \<and> ?P2 r'"
         proof(rule_tac x="(n_Exit  i)" in exI,rule conjI)
           show  "?P1 (n_Exit  i) " 
            by(cut_tac a1, auto) 
@@ -350,17 +928,17 @@ moreover{
            using lemmaOnn_ExitLeNc_ local.a1 a2 a4 a6 d0 by blast 
         qed
        }
-  ultimately show "∃r'.?P1 r' ∧ ?P2 r'" 
+  ultimately show "\<exists>r'.?P1 r' \<and> ?P2 r'" 
     by satx
 qed
 
 lemma lemmaOnn_IdleGt_i:
   assumes a1:"i>NC" and 
-  a2:"s ∈ reachableSet (set (allInitSpecs N)) (rules N)"  and a3:"NC<N" and  
-  a4:"∀f.  f ∈(set invariantsAbs) ⟶  formEval f s" 
+  a2:"s \<in> reachableSet (set (allInitSpecs N)) (rules N)"  and a3:"NC<N" and  
+  a4:"\<forall>f.  f \<in>(set invariantsAbs) \<longrightarrow>  formEval f s" 
   shows "trans_sim_on2 (n_Idle  i)  (n_Idle_i_3 ) VF (set invariantsAbs) s" (is "trans_sim_on2 ?r ?r' VF (set ?F) s")
   proof(rule ruleSimCond2)
-    show " formEval (pre ?r) s ⟶formEval (pre ?r') s" (is "?A ⟶?B")
+    show " formEval (pre ?r) s \<longrightarrow>formEval (pre ?r') s" (is "?A \<longrightarrow>?B")
     proof(rule impI)+
       assume b0:"?A"
   from a4  have tmp:"formEval (inv_27 0)  s"   
@@ -393,48 +971,48 @@ from a4  have tmp:"formEval (inv_5 0 1)  s"
        by auto
      qed
    next 
-	show "(∀  v. v ∈  varOfSent (act  ?r') ⟶  v ∈ VF ⟶ formEval (pre ?r) s ⟶ 
+	show "(\<forall>  v. v \<in>  varOfSent (act  ?r') \<longrightarrow>  v \<in> VF \<longrightarrow> formEval (pre ?r) s \<longrightarrow> 
     expEval (substExpByStatement (IVar v)  (act ?r')) s = expEval (substExpByStatement (IVar v)  (act ?r)) s)"
    proof(rule allI,(rule impI)+)
       fix  v
-     assume b1:"v∈ VF"  and b2:"formEval (pre ?r) s" and b3:"v ∈varOfSent (act ?r')"
+     assume b1:"v\<in> VF"  and b2:"formEval (pre ?r) s" and b3:"v \<in>varOfSent (act ?r')"
   
   show "expEval (substExpByStatement (IVar v)  (act ?r')) s = expEval (substExpByStatement (IVar v)  (act ?r)) s"  
        apply (cut_tac  a1 b1 b2 ,auto) done
    qed
  next
-   show "∀  v. v ∈  varOfSent (act ?r) ⟶  v ∈ VF ⟶ v ∈  varOfSent (act ?r')" by(cut_tac a1, auto)
+   show "\<forall>  v. v \<in>  varOfSent (act ?r) \<longrightarrow>  v \<in> VF \<longrightarrow> v \<in>  varOfSent (act ?r')" by(cut_tac a1, auto)
 
   
  next 
-   show "∀ v va. v ∈ varOfSent (act ?r') ⟶va∈varOfExp ( substExpByStatement (IVar v)  (act ?r'))⟶ va ∈ VF "
+   show "\<forall> v va. v \<in> varOfSent (act ?r') \<longrightarrow>va\<in>varOfExp ( substExpByStatement (IVar v)  (act ?r'))\<longrightarrow> va \<in> VF "
      by auto  
  next
-   show "∀v. v ∈ varOfForm (pre (?r')) ⟶ v ∈ VF" by auto
+   show "\<forall>v. v \<in> varOfForm (pre (?r')) \<longrightarrow> v \<in> VF" by auto
 qed
 lemma lemmaOnn_IdleLeNc_:
   assumes a1:"i\<le>NC" 
   shows "trans_sim_on2 (n_Idle  i) (n_Idle  i) VF  (set invariantsAbs) s" (is "trans_sim_on2 ?r ?r VF ?F s")
 proof(rule ruleSimId2)
-  show  "∀v. v∈varOfForm (pre ?r) ⟶  v ∈ VF "
+  show  "\<forall>v. v\<in>varOfForm (pre ?r) \<longrightarrow>  v \<in> VF "
     by(cut_tac a1, auto) 
     
 next
-  show  b1: "∀v a. a ∈ set (statement2Assigns (act ?r)) ⟶ v∈varOfExp ( substExpByStatement (IVar (fst a))  (act ?r))⟶v ∈VF "
+  show  b1: "\<forall>v a. a \<in> set (statement2Assigns (act ?r)) \<longrightarrow> v\<in>varOfExp ( substExpByStatement (IVar (fst a))  (act ?r))\<longrightarrow>v \<in>VF "
    proof(cut_tac a1,(rule allI)+,(rule impI)+,auto) qed
     
  qed
 lemma lemmaOnn_Idle: 
-  assumes   a2:"s ∈ reachableSet (set (allInitSpecs N)) (rules N)"  and  
-  a4:"∀f.  f ∈(set invariantsAbs) ⟶  formEval f s" and a5:"\<exists> i. i\<le>N\<and>r=n_Idle  i"  and
+  assumes   a2:"s \<in> reachableSet (set (allInitSpecs N)) (rules N)"  and  
+  a4:"\<forall>f.  f \<in>(set invariantsAbs) \<longrightarrow>  formEval f s" and a5:"\<exists> i. i\<le>N\<and>r=n_Idle  i"  and
   a6:"NC<N"
-  shows "∃ r'. r' ∈ rules NC∧ trans_sim_on2 r r' VF (set invariantsAbs) s" (is "∃r'.?P1 r' ∧ ?P2 r'")
+  shows "\<exists> r'. r' \<in> rules NC\<and> trans_sim_on2 r r' VF (set invariantsAbs) s" (is "\<exists>r'.?P1 r' \<and> ?P2 r'")
 proof -
   from a5 obtain i where d0:"i\<le>N\<and>r=n_Idle  i"  by blast
   have "i>NC|i\<le> NC" by auto
   moreover{
        assume a1:"i>NC" 
-        have "∃r'. ?P1 r' ∧ ?P2 r'"
+        have "\<exists>r'. ?P1 r' \<and> ?P2 r'"
         proof(rule_tac x="(n_Idle_i_3 )" in exI,rule conjI)
           show  "?P1 (n_Idle_i_3 ) " 
            by(cut_tac a1, auto) 
@@ -445,7 +1023,7 @@ proof -
        }
 moreover{
        assume a1:"i\<le> NC" 
-        have "∃r'. ?P1 r' ∧ ?P2 r'"
+        have "\<exists>r'. ?P1 r' \<and> ?P2 r'"
         proof(rule_tac x="(n_Idle  i)" in exI,rule conjI)
           show  "?P1 (n_Idle  i) " 
            by(cut_tac a1, auto) 
@@ -454,9 +1032,17 @@ moreover{
            using lemmaOnn_IdleLeNc_ local.a1 a2 a4 a6 d0 by blast 
         qed
        }
-  ultimately show "∃r'.?P1 r' ∧ ?P2 r'" 
+  ultimately show "\<exists>r'.?P1 r' \<and> ?P2 r'" 
     by satx
 qed
 
+definition n_Idle_PP::"nat \<Rightarrow> rule" where [simp]:
+"n_Idle_i_3PP i \<equiv> 
+let g = andForm (eqn (IVar (Para ( ''n'') i)) (Const E)) (andForm (andForm (eqn (IVar (Ident ''x'')) (Const false)) 
+(forallForm (down NC) (\<lambda>j. (neg (eqn (IVar (Para ( ''n'') j)) (Const E))))))
+ (forallForm (down NC) (\<lambda>j. (neg (eqn (IVar (Para ( ''n'') j)) (Const C)))))) in
+let s = (parallelList [(assign ((Ident ''x''), (Const true)))]) in
+guard g s"
 
+definition  NC::"nat " where [simp]: "NC==1"
 end
